Instantiated compiler model with PRNG

state/Examples.PRNG.fst
@@ -14,19 +14,22 @@ open Witnessable
 open Compiler
 open HigherOrderContracts
 open TargetLang
+open SpecTree
 
-assume val generate_nr : seed:int -> count:int -> int
+val generate_nr : seed:int -> count:int -> int
+let generate_nr seed count = seed+count
 
 let post = fun h0 _ h1 -> modifies_only_shared_and_encapsulated h0 h1 /\ gets_shared Set.empty h0 h1
 
 type prog_type =
-  seed:int -> SST (unit -> SST int (fun _ -> True) post) (fun _ -> True) post
+  seed:int -> SST (raise_t unit -> SST int (fun _ -> True) post) (fun _ -> True) post
 
-let prng (seed:int) : SST (unit -> SST int (fun _ -> True) post) (fun _ -> True) post =
+val prng : prog_type
+let prng (seed:int) =
   let counter : ref int = sst_alloc_shared 0 in
   witness (contains_pred counter) ;
   witness (is_shared counter) ;
-  fun () -> recall (contains_pred counter);
+  fun _ -> recall (contains_pred counter);
           recall (is_shared counter);
           let ccounter = sst_read counter in
           sst_write_shareable counter (ccounter + 1);
@@ -51,22 +54,36 @@ instance targetlang_arrow_helper pspec
   : targetlang pspec (raise_t unit -> SST int (fun _ -> True) post)
   = { wt = witnessable_arrow (raise_t unit) int _ _ }
 
-instance imp_prog : exportable_from prog_type = {
-  c_styp  = witnessable_arrow int  (unit -> SST int (fun _ -> True) post) _ _ ;
-  ityp = mk_interm_arrow int (raise_t unit -> SST int (fun _ -> True) post) ;
-  c_ityp = targetlang_arrow _ int (raise_t unit -> SST int (fun _ -> True) post) ;
-  export = (fun f z x -> f z (downgrade_val x)) ;
-  lemma_export_preserves_prref = (fun x -> ()) ;
-}
+instance exportable_prog pspec : exportable_from pspec (mk_targetlang_arrow pspec int (mk_targetlang_arrow pspec (raise_t unit) int)) Leaf =
+  targetlang_is_exportable _ pspec #(targetlang_arrow pspec int (mk_targetlang_arrow pspec (raise_t unit) int) #_ #(targetlang_arrow pspec (raise_t unit) int))
 
 let sit : src_interface2 = {
-  pt = prog_type ;
-  c_pt = solve ;
+  specs = (fun _ -> Leaf);
+  hocs = Leaf;
+  pt = (fun pspec -> mk_targetlang_arrow pspec int (mk_targetlang_arrow pspec (raise_t unit) int));
+  c_pt = (fun pspec -> exportable_prog pspec);
 }
 
+val prng' : prog_src2 sit
+let prng' seed =
+  let cb = prng seed in
+  (fun _ -> cb (raise_val ()))
 
 let compiled_prog =
-  compile_pprog2 #sit prng
+  compile_pprog2 #sit prng'
 
-let tmp = ctx_tgt2 (comp_int_src_tgt2 sit)
-// let mm = link_tgt2 compiled_prog single_use_caller
+val some_ctx : ctx_tgt2 (comp_int_src_tgt2 sit)
+let some_ctx inv prref hrel read write alloc prng =
+  let cb = prng 5 in
+  let _ = cb (raise_val ()) in
+  let _ = cb (raise_val ()) in
+  cb (raise_val ())
+
+let whole : whole_tgt2 =
+  link_tgt2 compiled_prog some_ctx
+
+let r = whole_prog ()
+let _ =
+  match r with
+  | 8 -> FStar.IO.print_string "Success"
+  | _ -> FStar.IO.print_string "Smething went wrong!"
